+ concept validity definitions

cpSTLC/cpSTLCa_Defs.v
@@ -11,8 +11,9 @@
 
 (* ***************************************************************** *)
 (** * cpSTLCa Syntax and Semantics Definition 
-      (Simply Typed Lambda Calculus with simple Concept Parameters  
-       :: version a) *)
+
+    (Simply Typed Lambda Calculus with simple Concept Parameters  
+     :: version a) *)
 (* ***************************************************************** *)
 (* ***************************************************************** *)
 
@@ -21,19 +22,26 @@ Add LoadPath "../..".
 Require Import ConceptParams.BasicPLDefs.Maps.
 Require Import ConceptParams.BasicPLDefs.Relations.
 
+Require Import Coq.Lists.List.
+Import ListNotations.
+
+Require Import Coq.omega.Omega.
+
 
 (* ################################################################# *)
 (** ** Syntax *)
 
-(** cpSTLCa -- Symply Typed Lambda Calculus 
-    with simple concept parameters.
-   
-    _Types_ are STLC types plus [C # T], 
-    where C is a concept name, T is a type.
-    
-    _Terms_ are STLC terms plus [\c#C. t], 
-    where c is a concept parameter.
+(** cpSTLCa — Symply Typed Lambda Calculus 
+    with simple _concept parameters_.
 
+
+    Types are STLC types with a type [C # T], 
+    where [C] is a concept name, [T] is a type.
+
+    Terms are STLC terms with a term [\c#C. t], 
+    where [c] is a concept parameter.
+
+<<
       CSec ::=           Concept declarations
              | <empty>              
              | CDef CSec           
@@ -83,22 +91,34 @@ Require Import ConceptParams.BasicPLDefs.Relations.
           | t t              function application
           | \c#C.t           concept parameter
           | t # M            model application
+          | c.f              concept element invocation
           | true
           | false
           | if t then t else t
           | n
           | succ t
           | pred t
+          | plus t t 
+          | minus t t 
           | mult t t   
+          | eqnat t t        nat equality
+          | le t t           nat less-than         
           | let x = t in t   let binding
+
+>>
 
     _Program_ consists of concept and model declarations, 
     and a term.
+
+<<
+      p ::=
+          | CSec MSec t
+>>
           
 *)
 
 (* ----------------------------------------------------------------- *)
-(** *** Types *)
+(** **** Types *)
 
 Inductive ty : Type :=
   | TBool : ty 
@@ -108,31 +128,44 @@ Inductive ty : Type :=
 .
 
 (* ----------------------------------------------------------------- *)
-(** *** Terms *)
+(** **** Terms *)
 
 Inductive tm : Type :=
   | tvar  : id -> tm               (* x *)
   | tapp  : tm -> tm -> tm         (* t1 t2 *)
   | tabs  : id -> ty -> tm -> tm   (* \x:T.t *)
   | tmapp : tm -> id -> tm         (* t # M *)
+  | tcabs  : id -> id -> tm -> tm  (* \c#C.t *)
+  | tcinvk : id -> id -> tm        (* c.f *)                                 
   | ttrue  : tm
   | tfalse : tm
   | tif : tm -> tm -> tm -> tm     (* if t1 then t2 else t3 *)
   | tnat   : nat -> tm             (* n *)
   | tsucc  : tm -> tm              (* succ t1 *) 
   | tpred  : tm -> tm              (* pred t1 *)
+  | tplus  : tm -> tm -> tm        (* plus t1 t2 *)
+  | tminus : tm -> tm -> tm        (* minus t1 t2 *)
   | tmult  : tm -> tm -> tm        (* mult t1 t2 *)
+  | teqnat : tm -> tm -> tm        (* eqnat t1 t2 *)
+  | tle    : tm -> tm -> tm        (* le t1 t2 *)
   | tlet   : id -> tm -> tm -> tm  (* let x = t1 in t2 *)                           
 .
 
 (* ----------------------------------------------------------------- *)
-(** *** Concepts *)
+(** **** Concepts *)
 
 (** Name declaration *)
 
 Inductive namedecl : Type :=
   | nm_decl : id -> ty -> namedecl   (* f : T *)
 .
+
+(** Auxiliary function to transform name declaration into pair *)
+Definition namedecl_to_pair (nmdecl : namedecl) : (id * ty) :=
+  match nmdecl with
+    nm_decl fname ftype => (fname, ftype)
+  end.
+
 
 (** List of name declarations *)
 
@@ -149,13 +182,19 @@ Inductive conceptdef : Type :=
 Definition conceptsec : Type := list conceptdef.
 
 (* ----------------------------------------------------------------- *)
-(** *** Models *)
+(** **** Models *)
 
 (** Name definition *)
 
 Inductive namedef : Type :=
   | nm_def : id -> tm -> namedef   (* f = T *)
 .
+
+(** Auxiliary function to transform name defintion into pair *)
+Definition namedef_to_pair (nmdef : namedef) : (id * tm) :=
+  match nmdef with
+    nm_def fname fdef => (fname, fdef)
+  end.
 
 (** List of name definitions *)
 
@@ -172,8 +211,261 @@ Inductive modeldef : Type :=
 Definition modelsec : Type := list modeldef.
 
 (* ----------------------------------------------------------------- *)
-(** *** Program *)
+(** **** Program *)
 
 Inductive program : Type :=
   | tprog : conceptsec -> modelsec -> tm -> program
 .
+
+(* ================================================================= *)
+(** *** Examples *)
+
+(** Let's define some examples so that we can check them later *)
+
+Module Examples.
+
+(** Concept names *)
+  
+Definition CNnrevmap := Id 1.
+Definition CNnmonoid := Id 2.
+Definition CNnfoo := Id 3.
+Definition CNbbar := Id 4.
+Definition CNempty := Id 5.
+
+(** Model names *)
+
+Definition MNnrm_plus1 := Id 11.
+Definition MNnrm_ident := Id 12.
+Definition MNnmnd_plus := Id 13.
+Definition MNnmnd_mult := Id 14.
+Definition MNnfoo := Id 15.
+Definition MNbbar1 := Id 16.
+Definition MNbbar2 := Id 17.
+
+(** Var names *)
+
+Definition vx := Id 30.
+Definition vy := Id 31.
+Definition vz := Id 32.
+
+(** Function names *)
+
+Definition FNmap := Id 40.
+Definition FNpam := Id 41.
+Definition FNident := Id 42.
+Definition FNop := Id 43.
+
+(** Concept definitions *)
+
+Definition Cnrevmap : conceptdef :=
+  cpt_def
+    (* name *) CNnrevmap
+    (* body *) [
+                 nm_decl FNmap (TArrow TNat TNat); (* map : Nat -> Nat  *)                    
+                 nm_decl FNpam (TArrow TNat TNat)  (* pam : Nat -> Nat  *)
+               ].
+          
+Definition Cnmonoid : conceptdef :=
+  cpt_def
+    (* name *) CNnmonoid
+    (* body *) [
+                 nm_decl FNident TNat;               (* ident : Nat   *)                    
+                 nm_decl FNop (TArrow TNat TNat)   (* op : Nat -> Nat -> Nat *)
+               ].
+
+Definition Cempty : conceptdef :=
+  cpt_def
+    (* name *) CNempty
+    (* body *) [].
+
+Definition Cbad1 : conceptdef :=
+  cpt_def
+    (* name *) CNnfoo
+    (* body *) [
+                 nm_decl FNmap (TArrow TNat TNat); (* map : Nat -> Nat  *)                    
+                 nm_decl FNmap (TArrow TNat TNat)  (* map : Nat -> Nat  *)
+               ].
+
+End Examples.
+
+
+(* ################################################################# *)
+(** ** Typing *)
+
+(** To typecheck terms with concept parameters, we need an additional 
+    context with information about concepts: concept context,
+    just st typing context.
+    
+    There must be a global _symbol table_ with information about
+    concepts and models.
+ *)
+
+(* ----------------------------------------------------------------- *)
+(** **** Checking Concept Definitions *)
+
+(** Concept information: list of pairs (element name, element type) 
+    [(fi, Ti)].
+ *)
+
+Definition cty : Type := list (id * ty).
+
+(** Concept definition is Ok if names of concept elements are
+    distinct, and types of elements are valid.
+
+    The only problem in types is with concept dependency [C # T]:
+    if C is undefined concept name, type is not valid.
+    So to check types validity, we need symbol table already.
+*)
+
+(** Symbol table is a map from concept names to concept types
+    [Ci -> CTi]. *)
+
+Definition symbtable : Type := partial_map cty.
+
+(** Now let's define a property "type is valid".
+    This property must be checked againts concrete symbol table.
+ *)
+
+Definition concept_defined (st :  symbtable) (C : id) : Prop := 
+  st C <> None.
+  
+Inductive ty_valid (st : symbtable) : ty -> Prop :=
+  | ty_valid_nat   : ty_valid st TNat
+  | ty_valid_bool  : ty_valid st TBool
+  | ty_valid_arrow : forall T1 T2,
+      ty_valid st T1 ->
+      ty_valid st T2 ->
+      ty_valid st (TArrow T1 T2)
+  | ty_valid_cpt   : forall C T,
+      concept_defined st C ->
+      ty_valid st T ->
+      ty_valid st (TConcept C T)
+.
+
+(** Now we are ready to define a property "concept is well defined" *)
+
+(*
+Print List.NoDup.
+Inductive NoDup (A : Type) : list A -> Prop :=
+    NoDup_nil : List.NoDup nil
+  | NoDup_cons : forall (x : A) (l : list A), ~ List.In x l -> List.NoDup l -> List.NoDup (x :: l)
+
+Print List.In.
+List.In = 
+fun A : Type =>
+fix In (a : A) (l : list A) {struct l} : Prop :=
+  match l with
+  | nil => False
+  | (b :: m)%list => b = a \/ In a m
+  end
+     : forall A : Type, A -> list A -> Prop
+
+Print List.Forall.
+Inductive Forall (A : Type) (P : A -> Prop) : list A -> Prop :=
+    Forall_nil : List.Forall P nil
+  | Forall_cons : forall (x : A) (l : list A), P x -> List.Forall P l -> List.Forall P (x :: l)
+*)
+
+Definition concept_welldefined (st : symbtable) (C : conceptdef) : Prop :=
+  match C with
+    cpt_def cname cbody =>
+    let (fnames, ftypes) := split (map namedecl_to_pair cbody) in
+    (** all names are distinct *)
+    List.NoDup fnames
+    (** and all types are valid *)
+    /\ List.Forall (fun ftype => ty_valid st ftype) ftypes            
+  end.
+  
+Definition stempty := @empty cty.
+
+(** Let's check some examples *)
+
+Module TestConcepts.
+Import Examples.
+  
+Example test_concept_1 : concept_welldefined stempty Cnrevmap.
+Proof.
+  unfold concept_welldefined, Cnrevmap.
+  simpl.
+  split.
+  - (* NoDup *)
+    apply NoDup_cons. intros H.
+    inversion H. inversion H0. inversion H0.
+    apply NoDup_cons. intros H. inversion H.
+    apply NoDup_nil.
+  - (* All types valid *)
+    apply Forall_cons. apply ty_valid_arrow; repeat constructor.
+    apply Forall_cons. apply ty_valid_arrow; repeat constructor.
+    apply Forall_nil.
+Qed.
+    
+End TestConcepts.
+
+
+(* ################################################################# *)
+(** ** Operational Semantics *)
+
+
+
+
+(* ================================================================= *)
+(** *** Substitution *)
+
+
+
+
+(*
+
+Fixpoint subst (x:id) (s:tm) (t:tm) : tm :=
+  match t with
+  | tvar y =>
+      if beq_id x y then s else t
+  | tabs y T t1 =>
+      tabs y T (if beq_id x y then t1 else (subst x s t1))
+  | tapp t1 t2 =>
+      tapp (subst x s t1) (subst x s t2)
+  | tnat n =>
+      tnat n
+  | tsucc t1 =>
+      tsucc (subst x s t1)
+  | tpred t1 =>
+      tpred (subst x s t1)
+  | tmult t1 t2 =>
+      tmult (subst x s t1) (subst x s t2)
+  | tif0 t1 t2 t3 =>
+      tif0 (subst x s t1) (subst x s t2) (subst x s t3)
+  | tpair t1 t2 =>
+      tpair (subst x s t1) (subst x s t2)
+  | tfst t1 =>
+      tfst (subst x s t1)
+  | tsnd t1 =>
+      tsnd (subst x s t1)
+  | tunit => tunit
+    (* [x := s] (let y = t1 in t2) *)           
+  | tlet y t1 t2 =>
+      tlet y (subst x s t1) (if beq_id x y then t2 else (subst x s t2))
+  | tinl T t1 =>
+      tinl T (subst x s t1)
+  | tinr T t1 =>
+      tinr T (subst x s t1)
+  | tcase t0 y1 t1 y2 t2 =>
+      tcase (subst x s t0)
+         y1 (if beq_id x y1 then t1 else (subst x s t1))
+         y2 (if beq_id x y2 then t2 else (subst x s t2))
+  | tnil T =>
+      tnil T
+  | tcons t1 t2 =>
+      tcons (subst x s t1) (subst x s t2)
+  | tlcase t1 t2 y1 y2 t3 =>
+      tlcase (subst x s t1) (subst x s t2) y1 y2
+        (if beq_id x y1 then
+           t3
+         else if beq_id x y2 then t3
+              else (subst x s t3))
+  | tfix t1 =>
+      tfix (subst x s t1)
+  end.
+
+Notation "'[' x ':=' s ']' t" := (subst x s t) (at level 20).
+
+ *)
